\documentclass[11pt]{article}

\usepackage{fullpage,graphicx,latexsym,picinpar,amsbsy,amsmath,amsfonts}

\input{macros.tex}

\begin{document}
	
% v -- YOUR NAME and SID in the braces
\student{ Nathan Ha}{ 862377326}  
% v -- YOUR NAME and SID in the braces
% \student{ name 2 }{sid 2 } 
% v -- ASSIGNMENT NUMBER in the braces
\assignment{ 3 } 
% v-- DUE DATE in the braces
\duedate{February 5, 2023 }  

\medskip

%%%%%%%%%%%%%%%%%%%%%%%%%%%%%%%%%%%%%%%%%%%%%%%%%%%%%%%%%%%%%%%%%%%%%%%%%%

\lineacross

%%%%%%%%%%%%%%%%%%%%%%%%%%%%
% problem 1
\begin{problem} \\
	\noindent a) Consider the following linear homogeneous recurrence relation: $R_n = 4R_{n-1} - 3R_{n-2}$. It is known that: $R_0 = 1$, $R_2 = 5$. Find $R_3$.

	\vspace {0.1in}
	\noindent b) Determine the general solution of the recurrence  equation if its characteristic equation has the following roots:  1, -2, -2, 2, 7, 7.

	\vspace {0.1in}
	\noindent  c) Determine the general solution of the recurrence  equation $A_n = 256A_{n-4}$.

	\vspace {0.1in}
	\noindent  d) Find the general form of the particular solution of the recurrence $B_n = 3B_{n-2} - 2B_{n-3}$ + 2.

\end{problem}

%---------------------------
% solution 1
\begin{solution} \\
	$(a)$ 
		This linear recurrence has a characteristic equation of $x^2 - 4x + 3 = 0$. This can be factored into $(x-3)(x-1) = 0 \implies x = 1, 3$. From here, we can write the general solution: \\ $R_n = \alpha_1(1)^n + \alpha_2(3)^n = \alpha_1 + \alpha_2(3)^n$. We can now plug in $R_0$ and $R_2$ to solve for $\alpha$. \\ $R_0 = 1 = \alpha_1 + \alpha_2$. \\ $R_2 = 5 = \alpha_1 + \alpha_2(3)^2$. \\ Solving this system of linear equations, we get $\alpha_{1,2} = \frac{1}{2}$. This means that the closed form for the recurrence is $R_n = \frac{1}{2}(3)^n + \frac{1}{2}$. We can plug in 3 and get $R_3 = \frac{1}{2}(3)^3 + \frac{1}{2} = 14$. 

	\text{}\\
	$(b)$
		A general solution of a recurrence with these roots would look like: \\ \text{}\quad\quad $R_n = \alpha_1(1)^n + \alpha_2(-2)^n + \alpha_3n(-2)^n + \alpha_4(2)^n + \alpha_5(7)^n + \alpha_6n(7)^n$.

	\text{}\\
	$(c)$
		The characteristic equation of this recurrence $x^4 - 256 = 0 \implies (x-4)(x+4)(x^2+16)=0 \\\implies (x-4)(x+4)(x+4i)(x-4i)=0$. The roots are $-4, 4, -4i, 4i$. The general solution to this is $R_n = \alpha_1(-4)^n + \alpha_2(4)^n + \alpha_3(-4i)^n + \alpha_4(4i)^n$.

	\text{}\\
	$(d)$
		TODO

	\end{solution}

%%%%%%%%%%%%%%%%%%%%%%%%%%%%
% problem 2
\newpage
\begin{problem}
	Solve the following recurrence equations:

%
$a)$
\begin{eqnarray*}
        f_n &=& f_{n-1} + 4f_{n-2} + 2f_{n-3}\\
        f_0 &=& 0 \\
        f_1 &=& 1 \\
		f_2 &=& 4 
\end{eqnarray*}
%
Show your work (all steps: the characteristic polynomial and its roots, the general solution, 
using the initial conditions to compute the final solution.)


$b)$
\begin{eqnarray*}
        t_n &=& t_{n-1} + 2t_{n-2} + 2^n\\
        t_0 &=& 0 \\
        t_1 &=& 2
\end{eqnarray*}
%
Show your work (all steps: the associated homogeneous equation,
the characteristic polynomial and its
roots, the general solution of the homogeneous
equation, computing a particular solution,
the general solution of the non-homogeneous equation,
using the initial conditions to compute the final solution.)
%
\end{problem}

%-----------------------------
% solution 2
\begin{solution} \\
	$(a)$ 
		The characteristic equation of this recurrence is $x^3 - x^2 -4x - 2 = 0$. Using the rational root theorem, we know that one root of this polynomial must be $\pm1$, or $\pm 2$. Pluggin in -1 yields a true statement, therefore we can factor out an $x+1$ from the characteristic equation. Using synthetic division, we get: $(x+1)(x^2 - 2x - 2) = 0$. Using the quadratic equation, we can simplify the second degree factor and get: $(x+1)(x - (1 - \sqrt{3}))(x-(1+ \sqrt{3})) = 0$. Now that we have the roots, we can find the general solution to the recurrence: $f_n = \alpha_1(-1)^n + \alpha_2(1 - \sqrt{3})^n + \alpha_3(1 + \sqrt{3})^n $. We can now plug in the base cases to solve for the constants: \\ $f_0 = 0 = \alpha_1 + \alpha_2 + \alpha_3$ \\ $ f_1 = 1 = -\alpha_1 + \alpha_2(1-\sqrt{3}) + \alpha_3(1+\sqrt{3}) $ \\ $ f_2 = 4 = \alpha_1 + \alpha_2(1-\sqrt{3})^2 + \alpha_3(1+\sqrt{3})^2 $ \\ Solving this system of linear equations gives $\alpha_{1,2,3} = 2, \frac{-6 - 5\sqrt{3}}{6}, \frac{-6 + 5\sqrt{3}}{6} $. Thus, the solution of the recurrence is $f_n = 2(-1)^n + \frac{-6 - 5\sqrt{3}}{6}(1 - \sqrt{3})^n + \frac{-6 + 5\sqrt{3}}{6}(1 + \sqrt{3})^n $.
\end{solution}

%%%%%%%%%%%%%%%%%%%%%%%%%%%
% problem 1
\newpage
\begin{problem}
 	PROBLEM 3 GOES HERE
\end{problem}

%----------------------------
% solution 3
\begin{solution}
	SOLUTION 3 GOES HERE
\end{solution}

\end{document}
